\section*{Chapter 2 - Random Variables}

\subsection*{Solution 1}

Let $x^+_1 > x^+_2 > ...$ and $x^-_1 < x^-_2 < ...$ such that $x^+_i \downarrow x$ and $x^-_i \uparrow x$.
Let $A_i = [x^-_i, x^+_i]$ for all $i > 0$.
Note that $A_{i+1} \subset A_i$ for all $i > 0$ and $A_i \to \{x\}$ as $i \to \infty$.
By theorem 1.8 (Continuity of Probability)
$$
P(x) = \lim_{i \to \infty} P(A_i) = \lim_{i \to \infty} (F(x^+_i) - F(x^-_i)) = F(x^+) - F(x^-).
$$

\subsection*{Solution 1 - Alternative}

By lemma 2.15.1 $P(x) = F(x) - F(x^-)$.
By Theorem 2.8.iii $F$ is right continuous, i.e. $F(x) = F(x^+)$, so $P(x) = F(x^+) - F(x^-)$.


\subsection*{Solution 2}

The CDF is given by
$$
F(x) = \left\{ \begin{array}{ll}
    0 & \text{if } x < 2, \\
    \frac{1}{10} & \text{if } 2 \leq x < 3, \\
    \frac{2}{10} & \text{if } 3 \leq x < 5, \\
    1 & \text{if } 5 \leq x
\end{array} \right.
$$
So $P(2 \leq X \leq 4.8) = F(4.8) - F(2^-) = \frac{2}{10}$.


\subsection*{Solution 3}

\begin{enumerate}
\item Let $x^-_1 < x^-_2 < ...$ such that $x^-_i \to x$ and $A_i = (x^-_i, x]$.
Then $A_i \supset A_{i+1}$ for all $i$ and $A_i \to \{x\}$.
By the continuity of the probability function
$$
P(x) = \lim_{i \to \infty} P(A_i) = \lim_{i \to \infty} F(x) - F(x^-_i) = F(x) - F(x^-).
$$
\item $P(x < X \leq y) = P(X \leq y) - P(X \leq x) = F(y) - F(x)$.
\item $P(X > x) = 1 - P(X \leq x) = 1 - F(x)$.
\item Follows directly from continuity of the probability function.
$P(x < X) = P(x \leq X)$ if $P$ is continuous.
\end{enumerate}


\subsection*{Solution 4}

(a)
$$
F_X(x) = \left\{ \begin{array}{ll}
    0 & \text{if } x \leq 0 \\
    x/4 & \text{if } 0 < x < 1 \\
    1/4 & \text{if } 1 \leq x \leq 3 \\
    1/8(3x - 7) & \text{if } 3 < x < 5 \\
    1 & \text{if } 5 \leq x
\end{array} \right.
$$

(b) For $Y = 1/X$, $F_Y(y) = P(1/X < y) = P(1/y < X) = 1 - P(X < 1/y)$, so
$$
F_Y(y) = \left\{ \begin{array}{ll}
    0 & \text{if } y < 1/5 \\
    1 - 1/8(3/y - 7) & \text{if } 1/5 \leq y < 1/3 \\
    3/4 & \text{if } 1/3 \leq y \leq 1 \\
    1 - 1/(4y) & \text{if } 1 < y
\end{array} \right.
$$


\subsection*{Solution 5}

Almost straight from the definition.
As $X$ and $Y$ are discrete random variables:
\begin{itemize}
\item[$\rightarrow$)] $f(x, y) = P(X \in \{x\}, Y \in \{y\}) = P(X \in \{x\})P(Y \in \{y\}) = f(x)f(y)$.
\item[$\leftarrow$)] $P(X \in A, Y \in B) = \sum_{(x, y) \in A \times B} f(x, y) = \sum_{x \in A} \sum_{y \in B} f(x) f(y) = P(X \in A) P(Y \in B)$.
\end{itemize}


\subsection*{Solution 6}

$Y = I_A(X)$ takes the value $1$ if $X \in A$ and $0$ if $X \notin A$.
So $P(Y = 0) = 1 - F_X(A)$ and $P(Y = 1) = F_X(A)$.
This gives the CDF
$$
F_Y(y) = \left\{ \begin{array}{ll}
    0 & \text{if } y < 0 \\
    1 - F_X(A) & \text{if } 0 \leq y < 1 \\
    1 & \text{if } 1 \leq y
\end{array} \right.
$$


\subsection*{Solution 7}

Let $Z = \mathrm{min}(X, Y)$, $X, Y \sim \mathrm{Uniform}(0, 1)$, then
\begin{equation*}
\begin{split}
F_Z(z) &= P(Z < z) \\
    &= 1 - P(Z > z) \\
    &= 1 - P(X > z \text{ and } Y > z) \\
    &= 1 - P(X > z)P(Y > z) \\
    &= 1 -(1 - F_X(z))(1 - F_Y(z))
    = 1 - (1 - z)^2.
\end{split}
\end{equation*}
Taking the derivative gives the probability distribution function
$$
f_Z(z) = 2 (1 - z).
$$


\subsection*{Solution 8}

Let $X$ be a random variable with CDF $F$.
Define $X^+ = \mathrm{max}(0, X)$.
Note that $P(X^+ < 0) = 0$ and $P(X^+ = 0) = P(X \leq 0) = F(0)$.
Therefore
\begin{equation*}
    F_+(x) = \left\{ \begin{array}{ll}
        0 & \text{if } x < 0 \\
        F(x) & \text{if } x \geq 0
    \end{array} \right.
\end{equation*}
